heap/pop/ret_path2_verif.v
@@ -1,0 +1,17 @@
+Require Import utils.VSTALib.
+
+Require Import heap.program.
+Require Import heap.definitions.
+Require Import heap.annotation.
+Require heap.pop.ret_path2.
+
+Module SH_Proof <: STRAIGHTLINE_HOARE_TRIPLE_PROOF.
+
+Include heap.pop.ret_path2.
+
+Theorem proof: functional_correctness_statement.
+Proof.
+  cbv delta [functional_correctness_statement].
+Admitted.
+
+End SH_Proof.
