heap/pop/verif.v
@@ -5,6 +5,7 @@ Require Import heap.definitions.
 Require Import heap.annotation.
 Require heap.pop.ret_path0_verif.
 Require heap.pop.ret_path1_verif.
+Require heap.pop.ret_path2_verif.
 
 Theorem f_pop_functionally_correct :
   semax_body Vprog Gprog f_pop pop_spec.
@@ -12,4 +13,5 @@ Proof.
   VST_A_start_function f_pop_hint.
   + apply ret_path0_verif.SH_Proof.proof.
   + apply ret_path1_verif.SH_Proof.proof.
+  + apply ret_path2_verif.SH_Proof.proof.
 Qed.
